Added x86 asmb and proof file with mc

x86/proofs/decode.ml
@@ -618,10 +618,22 @@ let decode_aux = new_definition `!pfxs rex l. decode_aux pfxs rex l =
     | VEXM_0F ->
         read_byte l >>= \(b,l).
         (bitmatch b with
+        | [0x12:8] ->
+          let sz = vexL_size L in
+          (read_ModRM rex l >>= \((reg,rm),l).
+            SOME (VMOVSLDUP (mmreg reg sz) (simd_of_RM sz rm),l))
         | [0x16:8] ->
           let sz = vexL_size L in
           (read_ModRM rex l >>= \((reg,rm),l).
             SOME (VMOVSHDUP (mmreg reg sz) (simd_of_RM sz rm),l))
+        | [0x6c:8] ->
+          let sz = vexL_size L in
+          (read_ModRM rex l >>= \((reg,rm),l).
+            SOME (VPUNPCKLQDQ (mmreg reg sz) (mmreg v sz) (simd_of_RM sz rm),l))
+        | [0x6d:8] ->
+          let sz = vexL_size L in
+          (read_ModRM rex l >>= \((reg,rm),l).
+            SOME (VPUNPCKHQDQ (mmreg reg sz) (mmreg v sz) (simd_of_RM sz rm),l))
         | [0x6f:8] ->
           let sz = vexL_size L in
           (read_ModRM rex l >>= \((reg,rm),l).
@@ -693,10 +705,30 @@ let decode_aux = new_definition `!pfxs rex l. decode_aux pfxs rex l =
               read_imm Byte l >>= (\(imm8,l).
               (let r3:3 word = word_zx reg in
               bitmatch r3 with
+              | [0b010:3] -> SOME (VPSRLQ (mmreg v sz) (simd_of_RM sz rm) imm8,l)
               | [0b110:3] -> SOME (VPSLLQ (mmreg v sz) (simd_of_RM sz rm) imm8,l)
               | _ -> NONE))
             | _ -> NONE)
           | _ -> NONE)
+    | VEXM_0F3A ->
+        read_byte l >>= \(b,l).
+        (bitmatch b with
+        | [0x00:8] ->
+          let sz = vexL_size L in
+          (read_ModRM rex l >>= \((reg,rm),l).
+          read_imm Byte l >>= \(imm8,l).
+            SOME (VPERMQ (mmreg reg sz) (simd_of_RM sz rm) imm8,l))
+        | [0x02:8] ->
+          let sz = vexL_size L in
+          (read_ModRM rex l >>= \((reg,rm),l).
+            read_imm Byte l >>= \(imm8,l).
+            SOME (VPBLENDD (mmreg reg sz) (mmreg v sz) (simd_of_RM sz rm) imm8,l))
+        | [0x46:8] ->
+          let sz = vexL_size L in
+          (read_ModRM rex l >>= \((reg,rm),l).
+          read_imm Byte l >>= \(imm8,l).
+            SOME (VPERM2I128 (mmreg reg sz) (mmreg v sz) (simd_of_RM sz rm) imm8,l))
+        | _ -> NONE)
     | _ -> NONE)
   | [0b1100011:7; v] -> if has_unhandled_pfxs pfxs then NONE else
     let sz = op_size_W rex v pfxs in
