x86/proofs/x86.ml
@@ -1327,6 +1327,19 @@ let x86_VMOVSHDUP = new_definition
           (word_zx x) in
         (dest := (word_zx res):N word) s`;;
 
+let x86_VMOVSLDUP = new_definition
+  `x86_VMOVSLDUP dest src (s:x86state) =
+      let (x:N word) = read src s in
+      if dimindex(:N) = 256 then
+        let res:(256)word = usimd4 (\(pair:64 word).
+          word_duplicate (word_subword pair (0,32):(32)word):(64)word)
+          (word_zx x) in
+        (dest := (word_zx res):N word) s
+      else
+        let res:(128)word = usimd2 (\(pair:64 word).
+          word_duplicate (word_subword pair (0,32):(32)word):(64)word)
+          (word_zx x) in
+        (dest := (word_zx res):N word) s`;;
 
 let x86_VPADDW = new_definition
   `x86_VPADDW dest src1 src2 (s:x86state) =
@@ -1349,13 +1362,76 @@ let x86_VPADDD = new_definition
       else
         let res:(128)word = simd4 word_add (word_zx x) (word_zx y) in
         (dest := (word_zx res):N word) s`;;
-        
+
+let msimd2 = new_definition
+ `(msimd2:(M word->N word->N word->N word)->
+        ((M)tybit0)word->((N)tybit0)word->((N)tybit0) word->((N)tybit0) word) f m x y =
+    word_join (f (word_subword m (dimindex(:M),dimindex(:M)))
+                 (word_subword x (dimindex(:N),dimindex(:N)))
+                 (word_subword y (dimindex(:N),dimindex(:N))))
+              (f (word_subword m (0,dimindex(:M)))
+                 (word_subword x (0,dimindex(:N)))
+                 (word_subword y (0,dimindex(:N))))`;;
+
+let msimd4 = new_definition
+ `msimd4 (f:M word->N word->N word->N word) = msimd2 (msimd2 f)`;;
+
+let msimd8 = new_definition
+ `msimd8 (f:M word->N word->N word->N word) = msimd2 (msimd4 f)`;;
+
+let msimd16 = new_definition
+ `msimd16 (f:M word->N word->N word->N word) = msimd2 (msimd8 f)`;;
+
+let x86_VPBLENDD = new_definition
+  `x86_VPBLENDD dest src1 src2 imm8 (s:x86state) =
+      let (x:N word) = read src1 s
+      and (y:N word) = read src2 s
+      and imm8 = read imm8 s in
+      let fn = \(i:1 word) (x:32 word) (y:32 word). if i = word 1 then y else x in
+      if dimindex(:N) = 256 then
+        let res:(256)word = msimd8 fn (word_zx imm8) (word_zx x) (word_zx y) in
+        (dest := (word_zx res):N word) s
+      else
+        let res:(128)word = msimd4 fn (word_zx imm8) (word_zx x) (word_zx y) in
+        (dest := (word_zx res):N word) s`;;
+
 let x86_VPBROADCASTD = new_definition
   `x86_VPBROADCASTD (dest:(x86state,(N)word)component) src (s:x86state) =
       let (x:128 word) = read src s in
       let dw = word_subword x (0,32):(32)word in
       let res:N word = word_duplicate dw in
       (dest := res) s`;;
+
+let x86_VPERMQ = new_definition
+  `x86_VPERMQ dest src imm8 (s:x86state) =
+      let (x:N word) = read src s
+      and od = read imm8 s in
+      if dimindex(:N) = 256 then
+        let res:(256)word = usimd4 (\(od:(2)word).
+            (word_subword:int256->num#num->int64) (word_zx x) ((val od)*64,64)) od in
+        (dest := (word_zx res):N word) s
+      else
+        raise_exception x86_Exception_UD s`;;
+
+let x86_VPERM2I128 = new_definition
+  `x86_VPERM2I128 dest src1 src2 imm8 (s:x86state) =
+      let (x1:N word) = read src1 s
+      and (x2:N word) = read src2 s
+      and od = read imm8 s in
+      if dimindex(:N) = 256 then
+        let res:(256)word = usimd2 (\(od:(4)word).
+            let sel = val od in
+            let zero_flag = (sel DIV 16) MOD 2 = 1 in
+            if zero_flag then (word 0):int128
+            else
+              let lane_sel = sel MOD 4 in
+              if lane_sel = 0 then (word_subword:int256->num#num->int128) (word_zx x1) (0,128)
+              else if lane_sel = 1 then (word_subword:int256->num#num->int128) (word_zx x1) (128,128)
+              else if lane_sel = 2 then (word_subword:int256->num#num->int128) (word_zx x2) (0,128)
+              else (word_subword:int256->num#num->int128) (word_zx x2) (128,128)) od in
+        (dest := (word_zx res):N word) s
+      else
+        raise_exception x86_Exception_UD s`;;
 
 let x86_VPMULDQ = new_definition
   `x86_VPMULDQ dest src1 src2 (s:x86state) =
@@ -1473,6 +1549,56 @@ let x86_VPSRLW = new_definition
         (dest := (word_zx res):N word) s
       else
         let res:(128)word = usimd8 (\z. word_ushr z count) (word_zx x) in
+        (dest := (word_zx res):N word) s`;;
+
+(* Only VPSRLQ version where shift count is an immediate value is supported *)
+let x86_VPSRLQ = new_definition
+  `x86_VPSRLQ dest src imm8 (s:x86state) =
+      let (x:N word) = read src s in
+      let count = val (read imm8 s) in
+      if dimindex(:N) = 256 then
+        let res:(256)word = usimd4 (\z. word_ushr z count) (word_zx x) in
+        (dest := (word_zx res):N word) s
+      else
+        let res:(128)word = usimd2 (\z. word_ushr z count) (word_zx x) in
+        (dest := (word_zx res):N word) s`;;
+
+let x86_VPUNPCKHQDQ = new_definition
+  `x86_VPUNPCKHQDQ dest src1 src2 (s:x86state) =
+      let (x:N word) = read src1 s
+      and (y:N word) = read src2 s in
+      if dimindex(:N) = 256 then
+        let x_low_high = (word_subword:int256->num#num->int64) (word_zx x) (64,64)
+        and x_high_high = (word_subword:int256->num#num->int64) (word_zx x) (192,64)
+        and y_low_high = (word_subword:int256->num#num->int64) (word_zx y) (64,64)
+        and y_high_high = (word_subword:int256->num#num->int64) (word_zx y) (192,64) in
+        let res = (word_join:int128->int128->int256)
+          ((word_join:int64->int64->int128) y_high_high x_high_high)
+          ((word_join:int64->int64->int128) y_low_high x_low_high) in
+        (dest := (word_zx res):N word) s
+      else
+        let x_high = (word_subword:int128->num#num->int64) (word_zx x) (64,64)
+        and y_high = (word_subword:int128->num#num->int64) (word_zx y) (64,64) in
+        let res = (word_join:int64->int64->int128) y_high x_high in
+        (dest := (word_zx res):N word) s`;;
+
+let x86_VPUNPCKLQDQ = new_definition
+  `x86_VPUNPCKLQDQ dest src1 src2 (s:x86state) =
+      let (x:N word) = read src1 s
+      and (y:N word) = read src2 s in
+      if dimindex(:N) = 256 then
+        let x_low = (word_subword:int256->num#num->int64) (word_zx x) (0,64)
+        and x_high = (word_subword:int256->num#num->int64) (word_zx x) (128,64)
+        and y_low = (word_subword:int256->num#num->int64) (word_zx y) (0,64)
+        and y_high = (word_subword:int256->num#num->int64) (word_zx y) (128,64) in
+        let res = (word_join:int128->int128->int256)
+          ((word_join:int64->int64->int128) y_high x_high)
+          ((word_join:int64->int64->int128) y_low x_low) in
+        (dest := (word_zx res):N word) s
+      else
+        let x_low = (word_subword:int128->num#num->int64) (word_zx x) (0,64)
+        and y_low = (word_subword:int128->num#num->int64) (word_zx y) (0,64) in
+        let res = (word_join:int64->int64->int128) y_low x_low in
         (dest := (word_zx res):N word) s`;;
 
 (*** This is roughly AND just for some condition codes ***)
@@ -2172,6 +2298,10 @@ let x86_execute = define
         (match operand_size dest with
           256 -> x86_VMOVSHDUP (OPERAND256 dest s) (OPERAND256 src s)
         | 128 -> x86_VMOVSHDUP (OPERAND128 dest s) (OPERAND128 src s)) s
+    | VMOVSLDUP dest src ->
+        (match operand_size dest with
+          256 -> x86_VMOVSLDUP (OPERAND256 dest s) (OPERAND256 src s)
+        | 128 -> x86_VMOVSLDUP (OPERAND128 dest s) (OPERAND128 src s)) s
     | VPADDW dest src1 src2 ->
         (match operand_size dest with
           256 -> x86_VPADDW (OPERAND256 dest s) (OPERAND256 src1 s) (OPERAND256 src2 s)
@@ -2180,10 +2310,22 @@ let x86_execute = define
         (match operand_size dest with
           256 -> x86_VPADDD (OPERAND256 dest s) (OPERAND256 src1 s) (OPERAND256 src2 s)
         | 128 -> x86_VPADDD (OPERAND128 dest s) (OPERAND128 src1 s) (OPERAND128 src2 s)) s
+    | VPBLENDD dest src1 src2 imm8 ->
+        (match operand_size dest with
+          256 -> x86_VPBLENDD (OPERAND256 dest s) (OPERAND256 src1 s) (OPERAND256 src2 s) (OPERAND8 imm8 s)
+        | 128 -> x86_VPBLENDD (OPERAND128 dest s) (OPERAND128 src1 s) (OPERAND128 src2 s) (OPERAND8 imm8 s)) s
     | VPBROADCASTD dest src ->
         (match operand_size dest with
           256 -> x86_VPBROADCASTD (OPERAND256 dest s) (OPERAND128 src s)
         | 128 -> x86_VPBROADCASTD (OPERAND128 dest s) (OPERAND128 src s)) s
+    | VPERMQ dest src imm8 ->
+        (match operand_size dest with
+          256 -> x86_VPERMQ (OPERAND256 dest s) (OPERAND256 src s) (OPERAND8 imm8 s)
+        | 128 -> x86_VPERMQ (OPERAND128 dest s) (OPERAND128 src s) (OPERAND8 imm8 s)) s
+    | VPERM2I128 dest src1 src2 imm8 ->
+        (match operand_size dest with
+          256 -> x86_VPERM2I128 (OPERAND256 dest s) (OPERAND256 src1 s) (OPERAND256 src2 s) (OPERAND8 imm8 s)
+        | 128 -> x86_VPERM2I128 (OPERAND128 dest s) (OPERAND128 src1 s) (OPERAND128 src2 s) (OPERAND8 imm8 s)) s
     | VPMULDQ dest src1 src2 ->
         (match operand_size dest with
           256 -> x86_VPMULDQ (OPERAND256 dest s) (OPERAND256 src1 s) (OPERAND256 src2 s)
@@ -2216,6 +2358,10 @@ let x86_execute = define
         (match operand_size dest with
           256 -> x86_VPSRAW (OPERAND256 dest s) (OPERAND256 src s) (OPERAND8 imm8 s)
         | 128 -> x86_VPSRAW (OPERAND128 dest s) (OPERAND128 src s) (OPERAND8 imm8 s)) s
+    | VPSRLQ dest src imm8 ->
+        (match operand_size dest with
+          256 -> x86_VPSRLQ (OPERAND256 dest s) (OPERAND256 src s) (OPERAND8 imm8 s)
+        | 128 -> x86_VPSRLQ (OPERAND128 dest s) (OPERAND128 src s) (OPERAND8 imm8 s)) s
     | VPSRLW dest src imm8 ->
         (match operand_size dest with
           256 -> x86_VPSRLW (OPERAND256 dest s) (OPERAND256 src s) (OPERAND8 imm8 s)
@@ -2232,6 +2378,14 @@ let x86_execute = define
         (match operand_size dest with
           256 -> x86_VPSRAD (OPERAND256 dest s) (OPERAND256 src s) (OPERAND8 imm8 s)
         | 128 -> x86_VPSRAD (OPERAND128 dest s) (OPERAND128 src s) (OPERAND8 imm8 s)) s
+    | VPUNPCKHQDQ dest src1 src2 ->
+        (match operand_size dest with
+          256 -> x86_VPUNPCKHQDQ (OPERAND256 dest s) (OPERAND256 src1 s) (OPERAND256 src2 s)
+        | 128 -> x86_VPUNPCKHQDQ (OPERAND128 dest s) (OPERAND128 src1 s) (OPERAND128 src2 s)) s
+    | VPUNPCKLQDQ dest src1 src2 ->
+        (match operand_size dest with
+          256 -> x86_VPUNPCKLQDQ (OPERAND256 dest s) (OPERAND256 src1 s) (OPERAND256 src2 s)
+        | 128 -> x86_VPUNPCKLQDQ (OPERAND128 dest s) (OPERAND128 src1 s) (OPERAND128 src2 s)) s
     | XCHG dest src ->
         (match operand_size dest with
           64 -> x86_XCHG (OPERAND64 dest s) (OPERAND64 src s)
@@ -2941,7 +3095,7 @@ let x86_RET_POP_RIP = prove
 (*** Simplify word operations in SIMD instructions ***)
 
 let all_simd_rules =
-   [usimd16;usimd8;usimd4;usimd2;simd16;simd8;simd4;simd2];;
+   [usimd16;usimd8;usimd4;usimd2;simd16;simd8;simd4;simd2;msimd16;msimd8;msimd4;msimd2];;
 
 let EXPAND_SIMD_RULE =
   CONV_RULE (TOP_DEPTH_CONV WORD_SIMPLE_SUBWORD_CONV) o
@@ -2954,9 +3108,13 @@ let x86_PSHUFD_ALT = EXPAND_SIMD_RULE x86_PSHUFD;;
 let x86_PSRAD_ALT = EXPAND_SIMD_RULE x86_PSRAD;;
 let x86_VMOVDQA_ALT = EXPAND_SIMD_RULE x86_VMOVDQA;;
 let x86_VMOVSHDUP_ALT = EXPAND_SIMD_RULE x86_VMOVSHDUP;;
+let x86_VMOVSLDUP_ALT = EXPAND_SIMD_RULE x86_VMOVSLDUP;;
 let x86_VPADDD_ALT = EXPAND_SIMD_RULE x86_VPADDD;;
 let x86_VPADDW_ALT = EXPAND_SIMD_RULE x86_VPADDW;;
+let x86_VPBLENDD_ALT = EXPAND_SIMD_RULE x86_VPBLENDD;;
 let x86_VPBROADCASTD_ALT = EXPAND_SIMD_RULE x86_VPBROADCASTD;;
+let x86_VPERMQ_ALT = EXPAND_SIMD_RULE x86_VPERMQ;;
+let x86_VPERM2I128_ALT = EXPAND_SIMD_RULE x86_VPERM2I128;;
 let x86_VPMULDQ_ALT = EXPAND_SIMD_RULE x86_VPMULDQ;;
 let x86_VPMULHW_ALT = EXPAND_SIMD_RULE x86_VPMULHW;;
 let x86_VPMULLD_ALT = EXPAND_SIMD_RULE x86_VPMULLD;;
@@ -2966,7 +3124,10 @@ let x86_VPSUBD_ALT = EXPAND_SIMD_RULE x86_VPSUBD;;
 let x86_VPSUBW_ALT = EXPAND_SIMD_RULE x86_VPSUBW;;
 let x86_VPSRAD_ALT = EXPAND_SIMD_RULE x86_VPSRAD;;
 let x86_VPSRAW_ALT = EXPAND_SIMD_RULE x86_VPSRAW;;
+let x86_VPSRLQ_ALT = EXPAND_SIMD_RULE x86_VPSRLQ;;
 let x86_VPSRLW_ALT = EXPAND_SIMD_RULE x86_VPSRLW;;
+let x86_VPUNPCKHQDQ_ALT = EXPAND_SIMD_RULE x86_VPUNPCKHQDQ;;
+let x86_VPUNPCKLQDQ_ALT = EXPAND_SIMD_RULE x86_VPUNPCKLQDQ;;
 
 
 let X86_OPERATION_CLAUSES =
@@ -2988,7 +3149,8 @@ let X86_OPERATION_CLAUSES =
     x86_VPADDD_ALT; x86_VPADDW_ALT; x86_VPMULHW_ALT; x86_VPMULLD_ALT; x86_VPMULLW_ALT;
     x86_VPSUBD_ALT; x86_VPSUBW_ALT; x86_VPXOR; x86_VPAND; x86_VPSRAD_ALT; x86_VPSRAW_ALT;
     x86_VPSRLW_ALT; x86_VPBROADCASTD_ALT; x86_VPSLLQ_ALT; x86_VMOVDQA_ALT; x86_VPMULDQ_ALT;
-    x86_VMOVSHDUP_ALT;
+    x86_VMOVSHDUP_ALT; x86_VPERMQ_ALT; x86_VPERM2I128_ALT; x86_VPUNPCKLQDQ_ALT; x86_VPUNPCKHQDQ_ALT;
+    x86_VMOVSLDUP_ALT; x86_VPBLENDD_ALT; x86_VPSRLQ_ALT;
     (*** 32-bit backups since the ALT forms are 64-bit only ***)
     INST_TYPE[`:32`,`:N`] x86_ADC;
     INST_TYPE[`:32`,`:N`] x86_ADCX;
